comprehensive

src/Experiments/Loops.v
@@ -12,346 +12,308 @@ Require Import Crypto.Util.LetIn.
 
 Require Import Crypto.Util.CPSNotations.
 
-(* TODO: do we have these anywhere? 
-Ltac forward H :=
-  match type of H with
-  | ?A -> ?B => let HA := fresh in assert A as HA; [|specialize(H HA)]
-  end.
-Ltac forward_by H t :=
-  match type of H with
-  | ?A -> ?B => let HA := fresh in assert A as HA by t; [|specialize(H HA)]
-  end.
- *)
+Module Import core.
+  Section Loops.
+    Context {A B : Type} (body : A -> A + B).
 
-Section Loops.
-  Context {A B : Type} (body : A -> A + B).
-
-  Fixpoint loop (fuel : nat) (s : A) {struct fuel} : A + B :=
-    match fuel with
-    | O => inl s
-    | S fuel' =>
-      let s := body s in
-      match s with
-      | inl a => loop fuel' a
-      | inr b => inr b
-      end
-    end.
-
-  Context (body_cps : A ~> A + B).
-
-  Fixpoint loop_cps (fuel : nat) (s : A) {struct fuel} :~> A + B :=
-    match fuel with
-    | O => return (inl s)
-    | S fuel' =>
-      s <- body_cps s;
+    Fixpoint loop (fuel : nat) (s : A) {struct fuel} : A + B :=
+      match fuel with
+      | O => inl s
+      | S fuel' =>
+        let s := body s in
         match s with
-        | inl a => loop_cps fuel' a
-        | inr b => return (inr b)
+        | inl a => loop fuel' a
+        | inr b => inr b
         end
-    end.
-
-  Context (body_cps_ok : forall s {R} f, body_cps s R f = f (body s)).
-  Lemma loop_cps_ok n s {R} f : loop_cps n s R f = f (loop n s).
-  Proof.
-    revert f; revert R; revert s; induction n; [reflexivity|]; cbn; intros.
-    cbv [cpscall cpsreturn]; rewrite body_cps_ok;
-      break_match; rewrite ?IHn; reflexivity.
-  Qed.
-
-  Context (body_cps2 : A -> forall {R}, (A -> R) -> (B -> R) -> R).
-  Fixpoint loop_cps2 (fuel : nat) (s : A) {R} (timeout:A->R) (ret:B->R) {struct fuel} : R :=
-    match fuel with
-    | O => timeout s
-    | S fuel' =>
-      body_cps2 s R
-                (fun a => @loop_cps2 fuel' a R timeout ret)
-                (fun b => ret b)
-    end.
-
-  Context (body_cps2_ok : forall s {R} continue break,
-              body_cps2 s R continue break =
-              match body s with
-              | inl a => continue a
-              | inr b => break b
-              end).
-  Lemma loop_cps2_ok n s {R} (timeout ret : _ -> R) :
-    @loop_cps2 n s R timeout ret =
-    match loop n s with
-    | inl a => timeout a
-    | inr b => ret b
-    end.
-  Proof.
-    revert ret; revert timeout; revert R; revert s;
-      induction n; intros; cbn; [reflexivity|].
-    rewrite body_cps2_ok.
-    destruct (body s); [|reflexivity].
-    rewrite IHn. reflexivity.
-  Qed.
-
-  Lemma loop_fuel_0 s : loop 0 s = inl s.
-  Proof. reflexivity. Qed.
-
-  Lemma loop_fuel_S_first n s : loop (S n) s =
-                                match body s with
-                                | inl a => loop n a
-                                | inr b => inr b
-                                end.
-  Proof. reflexivity. Qed.
-
-  Lemma loop_fuel_S_last n s : loop (S n) s =
-                          match loop n s with
-                          | inl a => body a
-                          | inr b => loop n s
-                          end.
-  Proof.
-    revert s; induction n; cbn; intros s.
-    { break_match; reflexivity. }
-    { destruct (body s); cbn; rewrite <-?IHn; reflexivity. }
-  Qed.
-
-  Lemma loop_fuel_S_stable n s b (H : loop n s = inr b) : loop (S n) s = inr b.
-  Proof.
-    revert H; revert b; revert s; induction n; intros ? ? H.
-    { cbn [loop nat_rect] in H. congruence_sum. }
-    { rewrite loop_fuel_S_last.
-      break_match; congruence_sum; reflexivity. }
-  Qed.
-
-  Lemma loop_fuel_add_stable n m s b (H : loop n s = inr b) : loop (m+n) s = inr b.
-  Proof.
-    induction m; intros.
-    { rewrite PeanoNat.Nat.add_0_l. assumption. }
-    { rewrite PeanoNat.Nat.add_succ_l.
-      erewrite loop_fuel_S_stable; eauto. }
-  Qed.
-
-  Lemma loop_fuel_irrelevant n m s bn bm
-        (Hn : loop n s = inr bn)
-        (Hm : loop m s = inr bm)
-    : bn = bm.
-  Proof.
-    destruct (Compare_dec.le_le_S_dec n m) as [H|H];
-      destruct (PeanoNat.Nat.le_exists_sub _ _ H) as [d [? _]]; subst.
-    { erewrite loop_fuel_add_stable in Hm by eassumption; congruence. }
-    { erewrite loop_fuel_add_stable in Hn.
-      { congruence_sum. reflexivity. }
-      { erewrite loop_fuel_S_stable by eassumption. congruence. } }
-  Qed.
-
-  Lemma by_invariant' (inv P:_->Prop) measure f s0
-          (inv_init : inv s0 /\ measure s0 < f)
-          (inv_continue : forall s s', body s = inl s' -> inv s -> inv s' /\ measure s' < measure s)
-          (inv_break : forall s s', body s = inr s' -> inv s -> P s')
-    : match loop f s0 with
-      | inl a => False
-      | inr s => P s
       end.
-  Proof.
-    revert dependent s0; induction f; intros; destruct_head'_and.
-    { exfalso; lia. }
-    { rewrite loop_fuel_S_first.
-      destruct (body s0) eqn:Hs0a; [|solve [eauto] ].
-      specialize (IHf a).
-      destruct (inv_continue s0 a Hs0a ltac:(assumption)).
-      specialize_by (split; (auto || lia)); auto. }
-  Qed.
 
-  Lemma by_invariant (inv P:_->Prop) measure f s0
-          (inv_init : inv s0 /\ measure s0 < f)
-          (inv_continue : forall s s', body s = inl s' -> inv s -> inv s' /\ measure s' < measure s)
-          (inv_break : forall s s', body s = inr s' -> inv s -> P s')
-    : exists b, loop f s0 = inr b /\ P b.
-  Proof.
-    pose proof (by_invariant' inv P measure f s0);
-      specialize_by assumption; break_match_hyps; [contradiction|eauto].
-  Qed.
+    Context (body_cps : A ~> A + B).
 
-  (* Completeness proof *)
+    Fixpoint loop_cps (fuel : nat) (s : A) {struct fuel} :~> A + B :=
+      match fuel with
+      | O => return (inl s)
+                  | S fuel' =>
+                    s <- body_cps s;
+                      match s with
+                      | inl a => loop_cps fuel' a
+                      | inr b => return (inr b)
+                      end
+      end.
 
-  Definition iterations_required fuel s : option nat :=
-    nat_rect _ None
-             (fun n r =>
-                match r with
-                | Some _ => r
-                | None =>
-                  match loop (S n) s with
-                  | inl a => None
-                  | inr b => Some (S n)
+    Context (body_cps_ok : forall s {R} f, body_cps s R f = f (body s)).
+    Lemma loop_cps_ok n s {R} f : loop_cps n s R f = f (loop n s).
+    Proof.
+      revert f; revert R; revert s; induction n; [reflexivity|]; cbn; intros.
+      cbv [cpscall cpsreturn]; rewrite body_cps_ok;
+        break_match; rewrite ?IHn; reflexivity.
+    Qed.
+
+    Context (body_cps2 : A -> forall {R}, (A -> R) -> (B -> R) -> R).
+    Fixpoint loop_cps2 (fuel : nat) (s : A) {R} (timeout:A->R) (ret:B->R) {struct fuel} : R :=
+      match fuel with
+      | O => timeout s
+      | S fuel' =>
+        body_cps2 s R
+                  (fun a => @loop_cps2 fuel' a R timeout ret)
+                  (fun b => ret b)
+      end.
+
+    Context (body_cps2_ok : forall s {R} continue break,
+                body_cps2 s R continue break =
+                match body s with
+                | inl a => continue a
+                | inr b => break b
+                end).
+    Lemma loop_cps2_ok n s {R} (timeout ret : _ -> R) :
+      @loop_cps2 n s R timeout ret =
+      match loop n s with
+      | inl a => timeout a
+      | inr b => ret b
+      end.
+    Proof.
+      revert ret; revert timeout; revert R; revert s;
+        induction n; intros; cbn; [reflexivity|].
+      rewrite body_cps2_ok.
+      destruct (body s); [|reflexivity].
+      rewrite IHn. reflexivity.
+    Qed.
+
+    Lemma loop_fuel_0 s : loop 0 s = inl s.
+    Proof. reflexivity. Qed.
+
+    Lemma loop_fuel_S_first n s : loop (S n) s =
+                                  match body s with
+                                  | inl a => loop n a
+                                  | inr b => inr b
+                                  end.
+    Proof. reflexivity. Qed.
+
+    Lemma loop_fuel_S_last n s : loop (S n) s =
+                                 match loop n s with
+                                 | inl a => body a
+                                 | inr b => loop n s
+                                 end.
+    Proof.
+      revert s; induction n; cbn; intros s.
+      { break_match; reflexivity. }
+      { destruct (body s); cbn; rewrite <-?IHn; reflexivity. }
+    Qed.
+
+    Lemma loop_fuel_S_stable n s b (H : loop n s = inr b) : loop (S n) s = inr b.
+    Proof.
+      revert H; revert b; revert s; induction n; intros ? ? H.
+      { cbn [loop nat_rect] in H. congruence_sum. }
+      { rewrite loop_fuel_S_last.
+        break_match; congruence_sum; reflexivity. }
+    Qed.
+
+    Lemma loop_fuel_add_stable n m s b (H : loop n s = inr b) : loop (m+n) s = inr b.
+    Proof.
+      induction m; intros.
+      { rewrite PeanoNat.Nat.add_0_l. assumption. }
+      { rewrite PeanoNat.Nat.add_succ_l.
+        erewrite loop_fuel_S_stable; eauto. }
+    Qed.
+
+    Lemma loop_fuel_irrelevant n m s bn bm
+          (Hn : loop n s = inr bn)
+          (Hm : loop m s = inr bm)
+      : bn = bm.
+    Proof.
+      destruct (Compare_dec.le_le_S_dec n m) as [H|H];
+        destruct (PeanoNat.Nat.le_exists_sub _ _ H) as [d [? _]]; subst.
+      { erewrite loop_fuel_add_stable in Hm by eassumption; congruence. }
+      { erewrite loop_fuel_add_stable in Hn.
+        { congruence_sum. reflexivity. }
+        { erewrite loop_fuel_S_stable by eassumption. congruence. } }
+    Qed.
+
+    Lemma by_invariant' (inv P:_->Prop) measure f s0
+          (init : inv s0 /\ measure s0 < f)
+          (step : forall s, inv s -> match body s with
+                                     | inl s' => inv s' /\ measure s' < measure s
+                                     | inr s' => P s'
+                                     end)
+      : match loop f s0 with
+        | inl a => False
+        | inr s => P s
+        end.
+    Proof.
+      revert dependent s0; induction f; intros; destruct_head'_and.
+      { exfalso; lia. }
+      { rewrite loop_fuel_S_first.
+        specialize (step s0 H); destruct (body s0); [|assumption].
+        destruct step.
+        exact (IHf a ltac:(split; (assumption || lia))). }
+    Qed.
+
+    Lemma by_invariant (inv P:_->Prop) measure f s0
+          (init : inv s0 /\ measure s0 < f)
+          (step : forall s, inv s -> match body s with
+                                     | inl s' => inv s' /\ measure s' < measure s
+                                     | inr s' => P s'
+                                     end)
+      : exists b, loop f s0 = inr b /\ P b.
+    Proof.
+      pose proof (by_invariant' inv P measure f s0);
+        specialize_by assumption; break_match_hyps; [contradiction|eauto].
+    Qed.
+
+    (* Completeness proof *)
+
+    Definition iterations_required fuel s : option nat :=
+      nat_rect _ None
+               (fun n r =>
+                  match r with
+                  | Some _ => r
+                  | None =>
+                    match loop (S n) s with
+                    | inl a => None
+                    | inr b => Some (S n)
+                    end
                   end
-                end
-             ) fuel.
+               ) fuel.
 
-  Lemma iterations_required_correct fuel s :
-    (forall m, iterations_required fuel s = Some m ->
-               1 <= m <= fuel /\
-      exists b, forall n, (n < m -> exists a, loop n s = inl a) /\ (m <= n -> loop n s = inr b))
+    Lemma iterations_required_correct fuel s :
+      (forall m, iterations_required fuel s = Some m ->
+                 1 <= m <= fuel /\
+                 exists b, forall n, (n < m -> exists a, loop n s = inl a) /\ (m <= n -> loop n s = inr b))
       /\
-    (iterations_required fuel s = None -> forall n, n <= fuel -> exists a, loop n s = inl a).
-  Proof.
-    induction fuel; intros.
-    { cbn. split; intros; inversion_option.
-      replace n with 0 by lia. rewrite loop_fuel_0. eauto. }
-    { change (iterations_required (S fuel) s)
-        with (match iterations_required fuel s with
-              | None => match loop (S fuel) s with
-                        | inl _ => None
-                        | inr _ => Some (S fuel)
-                        end
-              | Some _ => iterations_required fuel s
-              end) in *.
-      destruct (iterations_required fuel s) in *.
-      { split; intros; inversion_option; subst.
-        destruct (proj1 IHfuel _ eq_refl); split; [lia|assumption]. }
-      { destruct (loop (S fuel) s) eqn:HSf; split; intros; inversion_option; subst.
-        { intros. destruct (PeanoNat.Nat.eq_dec n (S fuel)); subst; eauto; [].
-          assert (n <= fuel) by lia. eapply IHfuel; congruence. }
-        { split; [lia|].
-          exists b; intros; split; intros.
-          { eapply IHfuel; congruence || lia. }
-          { eapply PeanoNat.Nat.le_exists_sub in H; destruct H as [?[]]; subst.
-            eauto using loop_fuel_add_stable. } } } }
-  Qed.
+      (iterations_required fuel s = None -> forall n, n <= fuel -> exists a, loop n s = inl a).
+    Proof.
+      induction fuel; intros.
+      { cbn. split; intros; inversion_option.
+        replace n with 0 by lia. rewrite loop_fuel_0. eauto. }
+      { change (iterations_required (S fuel) s)
+          with (match iterations_required fuel s with
+                | None => match loop (S fuel) s with
+                          | inl _ => None
+                          | inr _ => Some (S fuel)
+                          end
+                | Some _ => iterations_required fuel s
+                end) in *.
+        destruct (iterations_required fuel s) in *.
+        { split; intros; inversion_option; subst.
+          destruct (proj1 IHfuel _ eq_refl); split; [lia|assumption]. }
+        { destruct (loop (S fuel) s) eqn:HSf; split; intros; inversion_option; subst.
+          { intros. destruct (PeanoNat.Nat.eq_dec n (S fuel)); subst; eauto; [].
+            assert (n <= fuel) by lia. eapply IHfuel; congruence. }
+          { split; [lia|].
+            exists b; intros; split; intros.
+            { eapply IHfuel; congruence || lia. }
+            { eapply PeanoNat.Nat.le_exists_sub in H; destruct H as [?[]]; subst.
+              eauto using loop_fuel_add_stable. } } } }
+    Qed.
 
-  Lemma iterations_required_step fuel s s' n
-        (Hs : iterations_required fuel s = Some n)
-        (Hstep : body s = inl s')
-    : exists n', iterations_required fuel s' = Some n' /\ n = S n'.
-  Proof.
-    eapply iterations_required_correct in Hs.
-    destruct Hs as [Hn [b Hs]].
-    destruct n as [|n]; [pose proof (proj2 (Hs 0) ltac:(lia)) as Hx; inversion Hx|].
-    exists n; split; [|reflexivity].
-    pose proof (proj2 (Hs (S n)) ltac:(lia)) as H.
-    rewrite loop_fuel_S_first, Hstep in H.
-    destruct (iterations_required fuel s') as [x|] eqn:Hs' in *; [f_equal|exfalso].
-    { eapply iterations_required_correct in Hs'; destruct Hs' as [Hx Hs'].
-      destruct Hs' as [b' Hs'].
-      destruct (Compare_dec.le_lt_dec n x) as [Hc|Hc].
-      { destruct (Compare_dec.le_lt_dec x n) as [Hc'|Hc']; try lia; [].
-        destruct (proj1 (Hs' n) Hc'); congruence. }
-      { destruct (proj1 (Hs (S x)) ltac:(lia)) as [? HX].
-        rewrite loop_fuel_S_first, Hstep in HX.
-        pose proof (proj2 (Hs' x) ltac:(lia)).
-        congruence. } }
-    { eapply iterations_required_correct in Hs'; [|exact (ltac:(lia) : n <= fuel)].
-      destruct Hs'.
-      congruence. }
-  Qed.
+    Lemma iterations_required_step fuel s s' n
+          (Hs : iterations_required fuel s = Some n)
+          (Hstep : body s = inl s')
+      : exists n', iterations_required fuel s' = Some n' /\ n = S n'.
+    Proof.
+      eapply iterations_required_correct in Hs.
+      destruct Hs as [Hn [b Hs]].
+      destruct n as [|n]; [pose proof (proj2 (Hs 0) ltac:(lia)) as Hx; inversion Hx|].
+      exists n; split; [|reflexivity].
+      pose proof (proj2 (Hs (S n)) ltac:(lia)) as H.
+      rewrite loop_fuel_S_first, Hstep in H.
+      destruct (iterations_required fuel s') as [x|] eqn:Hs' in *; [f_equal|exfalso].
+      { eapply iterations_required_correct in Hs'; destruct Hs' as [Hx Hs'].
+        destruct Hs' as [b' Hs'].
+        destruct (Compare_dec.le_lt_dec n x) as [Hc|Hc].
+        { destruct (Compare_dec.le_lt_dec x n) as [Hc'|Hc']; try lia; [].
+          destruct (proj1 (Hs' n) Hc'); congruence. }
+        { destruct (proj1 (Hs (S x)) ltac:(lia)) as [? HX].
+          rewrite loop_fuel_S_first, Hstep in HX.
+          pose proof (proj2 (Hs' x) ltac:(lia)).
+          congruence. } }
+      { eapply iterations_required_correct in Hs'; [|exact (ltac:(lia) : n <= fuel)].
+        destruct Hs'.
+        congruence. }
+    Qed.
 
-  Lemma invariant_complete (P:_->Prop) f s0 b (H:loop f s0 = inr b) (HP:P b)
-        : exists inv measure,
-          (inv s0 /\ measure s0 < f)
-          /\ (forall s s', body s = inl s' -> inv s -> inv s' /\ measure s' < measure s)
-          /\ (forall s s', body s = inr s' -> inv s -> P s').
-  Proof.
-    set (measure f s :=
-           match iterations_required f s with
-           | None => 0
-           | Some s => pred s
-           end).
-    exists (fun s => match loop (S (measure f s)) s with
-                     | inl a => False
-                     | inr r => r = b end).
-    exists (measure f); split; [ |repeat match goal with |- _ /\ _ => split end..].
-    { cbv [measure].
-      destruct (iterations_required f s0) eqn:Hs0;
-        eapply iterations_required_correct in Hs0;
-          [ .. | exact (ltac:(lia):f <= f)]; [|destruct_head'_ex; congruence].
-      destruct Hs0 as [? [? Hs0]].
-      replace (S (Nat.pred n)) with n by lia.
-      pose proof (proj2 (Hs0 n) ltac:(lia)) as HH; rewrite HH.
-      split; [exact (loop_fuel_irrelevant _ _ _ _ _ HH H) | lia]. }
-    { intros s s' Hstep Hinv.
-      destruct (loop (S (measure f s)) s) eqn:Hs; [contradiction|subst].
-      cbv [measure] in *.
-      destruct (iterations_required f s) eqn:Hs' in *;
-       [|rewrite loop_fuel_S_last in Hs; cbv in Hs; congruence].
-      destruct (iterations_required_step _ _ s' _ Hs' Hstep) as [? [HA ?]]; subst.
-      rewrite HA.
-      destruct (proj1 (iterations_required_correct _ _) _ HA) as [? [? [? HE']]].
-      pose proof (HE' ltac:(constructor)) as HE; clear HE'.
-      split; [|lia].
-      replace (S (Nat.pred (S x))) with (S x) in * by lia.
-      rewrite loop_fuel_S_first, Hstep in Hs.
-      replace (S (Nat.pred x)) with x in * by lia; rewrite HE.
-      exact (loop_fuel_irrelevant _ _ _ _ _ HE Hs). }
-    { intros s c Hstep Hinv.
-      destruct (loop (S (measure f s)) s) eqn:Hs; [contradiction|subst].
-      assert (HH: loop 1 s = inr c) by (cbn; rewrite Hstep; reflexivity).
-      rewrite (loop_fuel_irrelevant _ _ _ _ _ HH Hs); exact HP. }
-  Qed.
-
-  Lemma invariant_iff f s0 P :
-    (exists b, loop f s0 = inr b /\ P b)
-    <->
-    (exists inv measure,
+    Lemma invariant_complete (P:_->Prop) f s0 b (H:loop f s0 = inr b) (HP:P b)
+      : exists inv measure,
         (inv s0 /\ measure s0 < f)
-        /\ (forall s s', body s = inl s' -> inv s -> inv s' /\ measure s' < measure s)
-        /\ (forall s s', body s = inr s' -> inv s -> P s')).
-  Proof.
-    repeat (intros || split || destruct_head'_ex || destruct_head'_and);
-      eauto using invariant_complete, by_invariant.
-  Qed.
+        /\ forall s, inv s -> match body s with
+                              | inl s' => inv s' /\ measure s' < measure s
+                              | inr s' => P s'
+                              end.
+    Proof.
+      set (measure f s :=
+             match iterations_required f s with
+             | None => 0
+             | Some s => pred s
+             end).
+      exists (fun s => match loop (S (measure f s)) s with
+                       | inl a => False
+                       | inr r => r = b end).
+      exists (measure f); split; [ |repeat match goal with |- _ /\ _ => split end..].
+      { cbv [measure].
+        destruct (iterations_required f s0) eqn:Hs0;
+          eapply iterations_required_correct in Hs0;
+          [ .. | exact (ltac:(lia):f <= f)]; [|destruct_head'_ex; congruence].
+        destruct Hs0 as [? [? Hs0]].
+        replace (S (Nat.pred n)) with n by lia.
+        pose proof (proj2 (Hs0 n) ltac:(lia)) as HH; rewrite HH.
+        split; [exact (loop_fuel_irrelevant _ _ _ _ _ HH H) | lia]. }
+      { intros s Hinv; destruct (body s) as [s'|c] eqn:Hstep.
+        { destruct (loop (S (measure f s)) s) eqn:Hs; [contradiction|subst].
+          cbv [measure] in *.
+          destruct (iterations_required f s) eqn:Hs' in *;
+            [|rewrite loop_fuel_S_last in Hs; cbv in Hs; congruence].
+          destruct (iterations_required_step _ _ s' _ Hs' Hstep) as [? [HA ?]]; subst.
+          rewrite HA.
+          destruct (proj1 (iterations_required_correct _ _) _ HA) as [? [? [? HE']]].
+          pose proof (HE' ltac:(constructor)) as HE; clear HE'.
+          split; [|lia].
+          replace (S (Nat.pred (S x))) with (S x) in * by lia.
+          rewrite loop_fuel_S_first, Hstep in Hs.
+          replace (S (Nat.pred x)) with x in * by lia; rewrite HE.
+          exact (loop_fuel_irrelevant _ _ _ _ _ HE Hs). }
+        { destruct (loop (S (measure f s)) s) eqn:Hs; [contradiction|subst].
+          assert (HH: loop 1 s = inr c) by (cbn; rewrite Hstep; reflexivity).
+          rewrite (loop_fuel_irrelevant _ _ _ _ _ HH Hs); exact HP. } }
+    Qed.
 
-  Lemma partial_by_invariant P inv f s0
-        (inv_init : inv s0)
-        (inv_continue : forall s s', body s = inl s' -> inv s -> inv s')
-        (inv_break : forall s s', body s = inr s' -> inv s -> P s')
-    : match loop f s0 with
-      | inl a => inv a
-      | inr s => P s
+    Lemma invariant_iff f s0 P :
+      (exists b, loop f s0 = inr b /\ P b)
+      <->
+      (exists inv measure,
+          (inv s0 /\ measure s0 < f)
+          /\ forall s, inv s -> match body s with
+                                | inl s' => inv s' /\ measure s' < measure s
+                                | inr s' => P s'
+                                end).
+    Proof.
+      repeat (intros || split || destruct_head'_ex || destruct_head'_and);
+        eauto using invariant_complete, by_invariant.
+    Qed.
+  End Loops.
+End core.
+
+Module default.
+  Section Default.
+    Context {A B} (default : B) (body : A -> A + B).
+    Definition loop fuel s : B :=
+      match loop body fuel s with
+      | inl s => default
+      | inr s => s
       end.
-  Proof.
-    induction f.
-    { rewrite loop_fuel_0; auto. }
-    { rewrite loop_fuel_S_last.
-      destruct (loop f s0) eqn:Hn;
-        [ destruct (body a) eqn:Ha; eauto | eauto ]. }
-  Qed.
 
-  Lemma by_invariant_inr P inv f s0 b (H : loop f s0 = inr b)
-          (inv_init : inv s0)
-          (inv_continue : forall s s', body s = inl s' -> inv s -> inv s')
-          (inv_break : forall s s', body s = inr s' -> inv s -> P s')
-      : P b.
-  Proof.
-    pose proof (partial_by_invariant P inv f s0) as HH.
-    rewrite H in HH; eauto.
-  Qed.
-
-  Lemma by_invariant_inr_complete (P:_->Prop) f s0 b (Hf : loop f s0 = inr b) (H : P b) :
-    exists (inv : A -> Prop),
-      inv s0
-      /\ (forall s s', body s = inl s' -> inv s -> inv s')
-      /\ (forall s s', body s = inr s' -> inv s -> P s').
-  Proof.
-    exists (fun s => exists n, match loop n s0 with
-                               | inl a => a = s
-                               | _ => False end).
-    repeat split.
-    { exists 0. rewrite loop_fuel_0. reflexivity. }
-    { intros s s' Hss' [n Hn]. exists (S n).
-      destruct (loop n s0) eqn:Hn_; [|contradiction]; subst a; rename Hn_ into Hn.
-      rewrite loop_fuel_S_last, Hn, Hss'. reflexivity. }
-    { intros s s' Hss' [n Hn].
-      destruct (loop n s0) eqn:Hn_; [|contradiction]; subst a; rename Hn_ into Hn.
-      assert (loop (S n) s0 = inr s') as HH by
-            (rewrite loop_fuel_S_last, Hn, Hss'; reflexivity).
-      rewrite (loop_fuel_irrelevant _ _ _ _ _ HH Hf); assumption. }
-  Qed.
-
-  Lemma invariant_inr_iff P f s0 b (H : loop f s0 = inr b) :
-      P b <->
-      (exists (inv : A -> Prop),
-          inv s0
-          /\ (forall s s', body s = inl s' -> inv s -> inv s')
-          /\ (forall s s', body s = inr s' -> inv s -> P s')).
-  Proof.
-    split.
-    { intros; eapply by_invariant_inr_complete; eauto. }
-    { intros [? [?[]]]; eapply by_invariant_inr; eauto. }
-  Qed.
-End Loops.
+    Lemma by_invariant inv (P:_->Prop) measure f s0
+          (init : inv s0 /\ measure s0 < f)
+          (step: forall s, inv s -> match body s with
+                                    | inl s' => inv s' /\ measure s' < measure s
+                                    | inr s' => P s'
+                                    end)
+      : P (loop f s0).
+    Proof.
+      edestruct (by_invariant body inv P measure f s0) as [x [HA HB]]; eauto; [].
+      apply (f_equal (fun r : A + B => match r with inl s => default | inr s => s end)) in HA.
+      cbv [loop]; break_match; congruence.
+    Qed.
+  End Default.
+End default.
 
 Module silent.
   Section Silent.
@@ -364,9 +326,10 @@ Module silent.
 
     Lemma by_invariant inv (P:_->Prop) measure f s0
           (init : inv s0 /\ measure s0 < f)
-          (step : forall s s' : state,
-              body s = inl s' -> inv s -> inv s' /\ measure s' < measure s)
-          (fini: forall s s' : state, body s = inr s' -> inv s -> P s')
+          (step: forall s, inv s -> match body s with
+                                    | inl s' => inv s' /\ measure s' < measure s
+                                    | inr s' => P s'
+                                    end)
       : P (loop f s0).
     Proof.
       edestruct (by_invariant body inv P measure f s0) as [x [A B]]; eauto; [].
@@ -391,33 +354,53 @@ Module while.
         else s
       end.
 
-    Section AsLoop.
-      Local Definition lbody := fun s => if test s then inl (body s) else inr s.
+    Local Definition lbody := fun s => if test s then inl (body s) else inr s.
 
-      Lemma eq_loop f s : while f s = sum_rect (fun _ => _) id id (loop lbody f s).
-      Proof.
-        revert s; induction f; intros s; [reflexivity|].
-        { cbv [lbody sum_rect id] in *; cbn in *.
-          rewrite IHf; break_innermost_match; reflexivity. }
-      Qed.
+    Lemma eq_loop f s : while f s = silent.loop lbody f s.
+    Proof.
+      revert s; induction f; intros s; [reflexivity|].
+      cbn; cbv [silent.loop lbody] in *.
+      rewrite IHf.
+      cbn; cbv [silent.loop lbody].
+      break_match; reflexivity.
+    Qed.
 
-      Lemma by_invariant inv P measure f s0
-            (init : inv s0 /\ measure s0 < f)
-            (step : forall s, if test s
-                              then inv s -> inv (body s) /\ measure (body s) < measure s
-                              else P (body s))
-        : P (while f s0).
-      Proof.
-      Qed.
-    End AsLoop.
+    Lemma by_invariant inv P measure f s0
+          (init : inv s0 /\ measure s0 < f)
+          (step : forall s, inv s -> if test s
+                                     then inv (body s) /\ measure (body s) < measure s
+                                     else P s)
+      : P (while f s0).
+    Proof.
+      rewrite eq_loop.
+      eapply silent.by_invariant; eauto; []; intros s H; cbv [lbody].
+      specialize (step s H); destruct (test s); eauto.
+    Qed.
+    
+    Context (body_cps : state ~> state).
+
+    Fixpoint while_cps f s :~> state :=
+      match f with
+      | O => return s
+      | S f =>
+        if test s
+        then s <- body_cps s; while_cps f s
+        else return s
+      end.
+
+    Context (body_cps_ok : forall s {R} f, body_cps s R f = f (body s)).
+    Lemma loop_cps_ok n s {R} f : while_cps n s R f = f (while n s).
+    Proof.
+      revert s; induction n; intros s; [reflexivity|].
+      cbn; break_match;
+        cbv [cpscall cpsreturn]; rewrite ?body_cps_ok, ?IHn; reflexivity.
+    Qed.
   End While.
-  Arguments by_invariant {_ _ _ _ _}.
 End while.
 Notation while := while.while.
 
 Definition for2 {state} (test : state -> bool) (increment body : state -> state)
-  := while test (fun s => increment (body s)). 
+  := while test (fun s => let s := body s in increment s). 
 
 Definition for3 {state} init test increment body fuel :=
   @for2 state test increment body fuel init.
-*)
